src/Convergence.v
@@ -7,7 +7,12 @@ Require Import Coq.Classes.Morphisms.
 Require Export Substitution.
 
 Definition conv {Var : Set} (x : Code Var) : Prop :=
-  exists y, probe x y /\ pi y TOP.
+  exists y, probe (close x) y /\ pi y TOP.
+
+Lemma conv_close (Var : Set) (x : Code Var) : conv (close x) <-> conv x.
+Proof.
+  unfold conv; code_simpl; tauto.
+Qed.
 
 Inductive prob {Var : Set} : Code Var -> Prop :=
   | prob_top : prob TOP
@@ -15,42 +20,72 @@ Inductive prob {Var : Set} : Code Var -> Prop :=
   | prob_r p q : prob p -> prob q -> prob (p (+) q).
 Hint Constructors prob.
 
-Definition pconv {Var : Set} (x p : Code Var) : Prop :=
-  prob p /\ exists y, probe x y /\ pi y p.
+Definition pconv {Var : Set} (x : Code Var) (p : Code Empty_set) : Prop :=
+  prob p /\ exists y, probe (x @ sub_top) y /\ pi y p.
+
+Ltac wlog_closed x :=
+  let cx := fresh "c" x in
+  let Ex := fresh "E" x in
+  let Hcx := fresh "H" cx in
+  rename x into cx;
+  assert (exists x, x = close cx) as Ex; [exists (close cx); reflexivity|];
+  destruct Ex as [x Ex];
+  assert (close x = x) as Hcx; [rewrite -> Ex; apply close_idempotent|];
+  repeat
+  match goal with
+    | [ H : conv x |- _] =>
+        rewrite <- conv_close in H;
+        replace (close cx) with x in H
+    | [|- conv x ] =>
+        rewrite <- conv_close;
+        replace (close cx) with x
+    | _ => idtac
+  end.
 
 Instance conv_proper_beta (Var : Set) :
   Proper (beta ==> iff) (@conv Var).
 Proof.
-  intros x x' xx'; split.
-  - intros [y [xy yt]].
+  intros x x' xx'; split; intro H;
+  wlog_closed x; wlog_closed x';
+  apply beta_close in xx'; rewrite <- Ex in xx'; rewrite <- Ex' in xx'.
+  - destruct H as [y [xy yt]].
+    rewrite <- Ex in xy.
     commute x' x y xx' xy as y'; exists y'.
-    split; auto.
+    split; [rewrite <- Ex'; auto|].
     rewrite <- (beta_pi_top _ _ _ y'y); auto.
-  - intros [y' [x'y' y't]].
+  - destruct H as [y' [x'y' y't]].
+    rewrite <- Ex' in x'y'.
     commute x x' y' xx' x'y' as y; exists y.
-    split; auto.
+    split; [rewrite <- Ex; auto|].
     transitivity y'; auto.
     rewrite yy'; auto.
 Qed.
 
 Instance conv_proper_pi (Var : Set) : Proper (pi --> impl) (@conv Var).
 Proof.
-  intros x x' xx' [y [xy yt]]; compute in xx'.
-    commute x' x y xx' xy as y'; exists y'.
-    split; auto.
-    transitivity y; auto.
+  intros x x' xx' [y [xy yt]];
+  wlog_closed x; wlog_closed x';
+  apply pi_close in xx'; rewrite <- Ex in xx'; rewrite <- Ex' in xx'.
+  rewrite <- Ex in xy.
+  commute x' x y xx' xy as y'; exists y'.
+  split; [rewrite <- Ex'; auto| eauto].
 Qed.
 
 Instance conv_proper_probe (Var : Set) : Proper (probe ==> iff) (@conv Var).
 Proof.
-  intros x x' xx'; split.
-  - intros [y [xy yt]].
+  intros x x' xx'; split; intro H;
+  wlog_closed x; wlog_closed x';
+  apply probe_close in xx'; rewrite <- Ex in xx'; rewrite <- Ex' in xx'.
+  - destruct H as [y [xy yt]].
+    rewrite <- Ex in xy.
     commute x' x y xx' xy as y'; exists y'.
-    repeat split; auto.
+    split; [rewrite <- Ex'; auto|].
     apply probe_pi_top with y; auto.
-  - intros [y' [x'y' y't]].
+  - destruct H as [y' [x'y' y't]].
     exists y'; split; auto.
+    rewrite <- Ex' in x'y'.
     transitivity x'; auto.
+    rewrite <- Ex; auto.
 Qed.
 
 Lemma conv_top (Var : Set) : conv (TOP : Code Var).
@@ -70,6 +105,12 @@ Ltac heads :=
   match goal with
   | [H : heads ?x ?y |- _] => inversion_clear H; heads
   end.
+
+Lemma heads_close (Var : Set) (h x : Code Var) :
+  heads h x -> heads (close h) (close x).
+Proof.
+  intro H; induction H; simpl; compute; heads.
+Qed.
 
 Lemma heads_probe (Var : Set) (h x y : Code Var) :
   probe x y -> heads h x -> heads h y.
@@ -93,6 +134,7 @@ Qed.
 Lemma not_conv_heads_bot (Var : Set) (x : Code Var) : heads BOT x -> ~ conv x.
 Proof.
   intros H [y [xy yt]].
+  apply (heads_close) in H.
   apply (heads_probe _ _ _ y) in H; auto.
   apply (heads_pi_bot _ _ TOP) in H; auto.
   inversion H; auto.
